iterators/hashtable_test.v
@@ -2,7 +2,144 @@ From iris.prelude Require Import listset_nodup.
 From iris.proofmode Require Import tactics.
 From iris.heap_lang Require Import lang notation proofmode.
 From iris.program_logic Require Import hoare.
-Require Import hashtable array.
+Require Import hashtable array util.
+
+
+Section TableInvariants.
+  Context `{Array Σ}.
+  Variable K : Hashable.
+
+  Existing Instances insertM key_eq.
+  
+  Lemma Forall_sublist {A} (l1 l2 : list A) P :
+    Forall P l1 ->
+    l2 `sublist_of` l1 ->
+    Forall P l2.
+  Proof.
+    intros HForall Hsub.
+    induction Hsub as [|x l1 l2 HSub IH|].
+    - done.
+    - apply Forall_cons in HForall. destruct HForall. auto using Forall_cons.
+    - apply Forall_cons in HForall. destruct HForall. auto.
+  Qed.
+
+  Lemma removal_sublist M seq M' k :
+    removal K M seq M' ->
+    M' k `sublist_of` M k.
+  Proof.
+    revert M M'. induction seq as [|[k' x] seq IH].
+    - intros M M' HRem. inversion HRem as [?? HM|]. simplify_eq. by rewrite HM. 
+    - intros M M' HRem. fold ([(k', x)] ++ seq) in HRem.
+      pose proof (removal_app_2 _ _ _ _ _ HRem) as [M'' [HRemkx ?]].
+      transitivity (M'' k) ; first by apply IH.
+      inversion HRemkx as [|????????? HM HRemnil]. simplify_eq.
+      inversion HRemnil as [?? HM'|]. rewrite -HM' HM /removeM. case_decide ; last done.
+      case (M k) ; first done. intros. by apply sublist_cons.
+  Qed.
+
+  Definition table_inv (P : val -> Prop) (M : Key K -> list val) : Prop :=
+    forall k, Forall  P (M k).
+
+  Lemma table_inv_empty P :
+    table_inv P (const []).
+  Proof.
+    intro. simpl. done.
+  Qed.
+  
+  Lemma table_inv_insert (P: val -> Prop) M k x :
+    P x -> table_inv P M -> table_inv P (<[k := x]>M).
+  Proof.
+    intros ?? k''. rewrite /base.insert /insertM. case_decide.
+    - simplify_eq. apply Forall_cons. eauto.
+    - done.
+  Qed.
+
+  Lemma table_inv_removal (P: val -> Prop) M M' seq :
+    table_inv P M -> removal K M seq M' -> Forall P (seq.*2).
+  Proof.
+    revert M.
+    induction seq as [|[k x] seq IH] ; first (intros ; by apply Forall_nil).
+    rewrite -/([(k, x)] ++ seq) fmap_app. intros M HInv HRem.
+    pose proof (removal_app_2 _ _ _ _ _ HRem) as [M'' [HRemkx ?]].
+    apply Forall_app. split.
+    - inversion HRemkx as [|? k' ????? HKk HMk]. simplify_eq. 
+      assert (exists l, M k' = x :: l) as [l Hl].
+      { unfold hd_error in HMk. destruct (M k'). discriminate. eexists. injection HMk. by intros ->. }
+      specialize (HInv k'). rewrite Hl in HInv. apply Forall_cons in HInv.
+      destruct HInv as [? _]. by apply Forall_singleton.  
+    - apply (IH M'') ; last assumption. intro k'. apply (Forall_sublist (M k')) ; first done. by eapply removal_sublist.
+  Qed.
+
+    Definition elementsM (M: Key K -> list val) (D: listset_nodup (Key K)) :=
+    collection_fold (fun k l => M k ++ l) [] D.
+
+  Instance elementsM_proper M : Proper ((≡) ==> (≡ₚ)) (elementsM M).
+  Proof.
+    apply collection_fold_proper. typeclasses eauto. solve_proper.
+    intros. do 2 rewrite app_assoc. apply Permutation_app. apply Permutation_app_comm. reflexivity.
+  Qed.
+      
+      
+  Lemma elementsM_insert M D k x:
+    is_domain K D M ->
+    elementsM (<[k := x]>M) ({[k]} ∪ D) ≡ₚ x :: elementsM M D.
+  Proof.
+    assert (forall M, Proper ((=) ==> (≡ₚ) ==> (≡ₚ)) (λ (k : Key K) (l : list val), M k ++ l)) ; first solve_proper.
+    assert (forall A (l1 l2 l3 : list A), l1 ++ l2 ++ l3 ≡ₚ l2 ++ l1 ++ l3).
+    { intros. do 2 rewrite app_assoc. apply Permutation_app. apply Permutation_app_comm. reflexivity. }
+    intro Hdom.
+    destruct (decide (k ∈ D)).
+    - rewrite subseteq_union_1 ; last by apply elem_of_subseteq_singleton.
+      rewrite (union_difference {[k]} D) ; last by apply elem_of_subseteq_singleton.
+      rewrite /elementsM.
+      erewrite collection_fold_union_singleton ; [|typeclasses eauto|done..|set_solver].
+      erewrite collection_fold_union_singleton ; [|typeclasses eauto|done..|set_solver].
+      rewrite /base.insert /insertM decide_True /= ; last reflexivity.
+      do 2 f_equiv. apply collection_fold_domains ; [typeclasses eauto.. |done|done|].
+      intros. rewrite decide_False. by f_equiv. set_solver.
+    - rewrite /elementsM.
+      erewrite collection_fold_union_singleton ; [|typeclasses eauto|done..|set_solver].
+      rewrite /base.insert /insertM decide_True /= ; last reflexivity.
+      rewrite Hdom /=; last assumption. f_equiv.
+      apply collection_fold_domains ; [typeclasses eauto.. |done|done|].
+      intros. rewrite decide_False. by f_equiv. set_solver.
+  Qed.
+
+  Lemma elementsM_complete_permutation M D seq:
+    is_domain K D M ->
+    complete K M seq ->
+    seq.*2 ≡ₚ elementsM M D.
+  Proof.
+    revert M.
+    induction seq as [|[k x] seq IH].
+    - intros M Hdom HCom. inversion HCom as [???HM|]. Check collection_fold_ind.
+      apply (collection_fold_ind (fun seq D => is_domain _ D M -> [] ≡ₚ seq)).
+      + by intros ?? <- ?? <-.
+      + reflexivity.
+      + intros ???? IH ?. rewrite HM. apply IH. intros ??. by rewrite HM.
+      + done.
+    - intros M Hdom HCom. inversion HCom as [|??k'??? M' ?? Hx HM'].
+      assert (is_domain K D M').
+      { intros ??. rewrite HM'. unfold removeM. case_decide ; by rewrite Hdom. }
+      assert (HMM' : forall k, M k = (<[k' := x]>M') k).
+      {
+        unfold base.insert, insertM.
+        intro k''. rewrite HM'. unfold removeM. case_decide.
+        simplify_eq. destruct (M k''). discriminate. injection Hx. by intros <-. done.
+      }
+      
+      assert (Heq : elementsM M D ≡ₚ x :: elementsM M' D).
+      { rewrite -(elementsM_insert _ _ k'). rewrite (_:{[k']} ∪ D ≡ D).
+        unfold elementsM. apply collection_fold_domains ;
+        [typeclasses eauto| solve_proper| solve_proper|
+         (intros ; do 2 rewrite app_assoc ; f_equiv ; apply Permutation_app_comm) .. |].
+        intros ??? <- ?. by rewrite HMM'.
+        destruct (decide (k' ∈ D)). set_solver. rewrite Hdom in Hx. discriminate. assumption. assumption.
+      }
+      rewrite Heq fmap_cons /=. f_equiv. by apply IH.
+  Qed.
+  
+End TableInvariants.
 
 Section Tests.
   Context `{Array Σ}.
@@ -40,14 +177,9 @@ Section Tests.
   Proof.
     intro. wp_lam. eauto using as_natkey_inj.
   Qed.
-  
-  Print Hashable.
-  
+    
   Definition nat_hashable : Hashable :=
     {| equal_spec := equalf_spec ; hash_spec := idhash_spec  |}.
-
-  Check insert_impl.
-
   
   Variable modulo: val.
   
@@ -71,171 +203,65 @@ Section Tests.
     insert "t" #1 #1 ;;
     insert "t" #2 #2 ;;
     let: "a" := ref #0 in      
-    fold_impl (λ: "k" "x", "a" <- !"a" + "x") "t" #() ;;
+    fold_impl (λ: "k" "x" <>, "a" <- !"a" + "x") "t" #() ;;
     !"a".
 
   Definition permitted := permitted nat_hashable.
   Definition complete := complete nat_hashable.
 
-  Definition elementsM (M: nat -> list val) (D: listset_nodup nat) :=
-    collection_fold (fun k l => M k ++ l) [] D.
-
-  Instance elementsM_proper M : Proper ((≡) ==> (≡ₚ)) (elementsM M).
-  Proof.
-    apply collection_fold_proper. typeclasses eauto. solve_proper.
-    intros. do 2 rewrite app_assoc. apply Permutation_app. apply Permutation_app_comm. reflexivity.
-  Qed.
-
-  Lemma collection_fold_union_singleton `{FinCollection A C} {B} f (b : B) (x : A) (X : C)
-        `{!Equivalence R} `{!Proper ((=) ==> R ==> R) f} :
-    (∀ a1 a2 b, R (f a1 (f a2 b)) (f a2 (f a1 b))) ->
-    x ∉ X ->
-    R (collection_fold f b ({[x]} ∪ X)) (f x (collection_fold f b X)).
-  Proof.
-    assert (HProper: Proper (eq ==> R ==> R) f) ; first assumption.
-    intros Hf ?.
-    rewrite /collection_fold /=.
-    assert (Proper ((≡ₚ) ==> R) (foldr f b)).
-    { intro. apply foldr_permutation. typeclasses eauto. intro. by apply HProper. assumption. }
-    rewrite elements_union_singleton /=; last assumption. reflexivity.
-  Qed.
-
-  Lemma collection_fold_with_domains `{FinCollection A C} {B} (b : B) X f g `{!Equivalence R}
-        `{!Proper ((=) ==> R ==> R) f} `{!Proper ((=) ==> R ==> R) g}:
-    (∀ a1 a2 b, R (f a1 (f a2 b)) (f a2 (f a1 b))) ->
-    (∀ a1 a2 b, R (g a1 (g a2 b)) (g a2 (g a1 b))) ->
-   (forall a b1 b2, R b1 b2 -> a ∈ X -> R (f a b1) (g a b2)) ->
-   R (collection_fold f b X) (collection_fold g b X).
-  Proof.
-    intros.
-    apply (collection_ind
-             (fun X => (forall a b1 b2, R b1 b2 -> a ∈ X -> R (f a b1) (g a b2)) ->
-                       R (collection_fold f b X) (collection_fold g b X))) ; last assumption.
-    {
-      intros ?? Heq. rewrite (collection_fold_proper _ _ _ _ _ _ Heq).
-      rewrite (collection_fold_proper _ _ _ _ _ _ Heq).
-      split ; intros Hyp ? ; apply Hyp ; intros ???? ; [rewrite Heq |rewrite -Heq] ; eauto.
-      all : assumption.
-    }
-    - intros. by rewrite /collection_fold /= elements_empty. 
-    - intros ??? IH Hfg.
-      rewrite collection_fold_union_singleton ; [|assumption..].
-      rewrite collection_fold_union_singleton ; [|assumption..].
-      apply Hfg. apply IH. intros. apply Hfg. assumption. all: set_solver.
-  Qed.
-      
-      
-  Lemma elementsM_insert M D k x:
-    is_domain nat_hashable D M ->
-    elementsM (<[k := x]>M) ({[k]} ∪ D) ≡ₚ x :: elementsM M D.
-  Proof.
-    assert (forall M, Proper ((=) ==> (≡ₚ) ==> (≡ₚ)) (λ (k0 : nat) (l : list val), M k0 ++ l)) ; first solve_proper.
-    assert (forall A (l1 l2 l3 : list A), l1 ++ l2 ++ l3 ≡ₚ l2 ++ l1 ++ l3).
-    { intros. do 2 rewrite app_assoc. apply Permutation_app. apply Permutation_app_comm. reflexivity. }
-    intro Hdom.
-    destruct (decide (k ∈ D)).
-    - rewrite subseteq_union_1 ; last by apply elem_of_subseteq_singleton.
-      rewrite (union_difference {[k]} D) ; last by apply elem_of_subseteq_singleton.
-      rewrite /elementsM.
-      erewrite collection_fold_union_singleton ; [|typeclasses eauto|done..|set_solver].
-      erewrite collection_fold_union_singleton ; [|typeclasses eauto|done..|set_solver].
-      rewrite /base.insert /insertM_nat /insertM decide_True /= ; last reflexivity.
-      do 2 f_equiv. apply collection_fold_with_domains ; [typeclasses eauto.. |done|done|].
-      intros. rewrite decide_False. by f_equiv. set_solver.
-    - rewrite /elementsM.
-      erewrite collection_fold_union_singleton ; [|typeclasses eauto|done..|set_solver].
-      rewrite /base.insert /insertM_nat /insertM decide_True /= ; last reflexivity.
-      rewrite Hdom /=; last assumption. f_equiv.
-      apply collection_fold_with_domains ; [typeclasses eauto.. |done|done|].
-      intros. rewrite decide_False. by f_equiv. set_solver.
-  Qed.
       
   
-  Definition int_table (M : nat -> list val) :=
-    forall i, Forall (fun v => exists (j : Z), v = #j) (M i).
-
-  Lemma Forall_sublist {A} (l1 l2 : list A) P :
-    Forall P l1 ->
-    l2 `sublist_of` l1 ->
-    Forall P l2.
-  Proof.
-    intros HForall Hsub.
-    induction Hsub as [|x l1 l2 HSub IH|].
-    - done.
-    - apply Forall_cons in HForall. destruct HForall. auto using Forall_cons.
-    - apply Forall_cons in HForall. destruct HForall. auto.
-  Qed.
-
-  Lemma removal_sublist K M seq M' k :
-    removal K M seq M' ->
-    M' k `sublist_of` M k.
-  Proof.
-    revert M M'. induction seq as [|[k' x] seq IH].
-    - intros M M' HRem. inversion HRem as [?? HM|]. simplify_eq. by rewrite HM. 
-    - intros M M' HRem. fold ([(k', x)] ++ seq) in HRem.
-      pose proof (removal_app_2 _ _ _ _ _ HRem) as [M'' [HRemkx ?]].
-      transitivity (M'' k) ; first by apply IH.
-      inversion HRemkx as [|????????? HM HRemnil]. simplify_eq.
-      inversion HRemnil as [?? HM'|]. rewrite -HM' HM /removeM. case_decide ; last done.
-      case (M k) ; first done. intros. by apply sublist_cons.
-  Qed.
-      
-  Lemma int_table_permitted M seq :
-    int_table M ->
-    permitted M seq ->
-    Forall (fun v => exists (j : Z), v = #j) (seq.*2).
-  Proof.
-    revert M.
-    induction seq as [|[k x] seq IH] ; first (intros ; by apply Forall_nil).
-    rewrite -/([(k, x)] ++ seq) fmap_app. intros M HiTab HPer.
-    destruct HPer as [M' HRem]. pose proof (removal_app_2 _ _ _ _ _ HRem) as [M'' [HRemkx ?]].
-    apply Forall_app. split.
-    - inversion HRemkx as [|? k' ????? HKk HMk]. simplify_eq. 
-      assert (exists l, M k' = x :: l) as [l Hl].
-      { unfold hd_error in HMk. destruct (M k'). discriminate. eexists. injection HMk. by intros ->. }
-      specialize (HiTab k'). rewrite Hl in HiTab. apply Forall_cons in HiTab.
-      destruct HiTab as [? _]. by apply Forall_singleton.  
-    - apply (IH M''). intro k'. apply (Forall_sublist (M k')) ; first done. by eapply removal_sublist.
-      by exists M'.
-  Qed.            
+  Definition int_table :=
+    table_inv nat_hashable (fun v => exists (j : Z), v = #j).
     
-  Fixpoint table_seq_sum (seq : list (val * val)) :=
+  Fixpoint table_seq_sum (seq : list (val)) :=
     match seq with
     | [] => Some 0%Z
-    | (k, #(LitInt x)) :: seq => z ← table_seq_sum seq ; Some (z + x)%Z
+    |  #(LitInt x) :: seq => z ← table_seq_sum seq ; Some (z + x)%Z
     | _ => None
     end.
+
+  Instance table_seq_sum_proper : Proper ((≡ₚ) ==> (=)) table_seq_sum.
+  Proof.
+    induction 1 as[|x|x y l| ???? Heq1 ? Heq2]. reflexivity.
+    - destruct x as [|x| | |]; try reflexivity. destruct x as [n| | |] ; try reflexivity.
+      simpl. by f_equal.
+    - destruct x as [|x| | |]; cycle 1 ; [destruct x|..] ; (destruct y as [|y| | |] ; cycle 1 ; [destruct y|..]) ; try reflexivity.
+      simpl. destruct (table_seq_sum l) ; last reflexivity. simpl. f_equal. lia.
+    - by rewrite Heq1.
+  Qed.
+    
 
   Lemma table_seq_sum_app seq seq':
     table_seq_sum (seq ++ seq') = x ← table_seq_sum seq ; y ← table_seq_sum seq' ; Some (x + y)%Z.
   Proof.
-    induction seq as [| [? x] seq IH]. simpl. rewrite /mbind /option_bind ; by destruct (table_seq_sum seq').
+    induction seq as [|x seq IH]. simpl. rewrite /mbind /option_bind ; by destruct (table_seq_sum seq').
     destruct x as [|x | | |] ; try reflexivity. destruct x ; try reflexivity.
     simpl. rewrite IH. destruct (table_seq_sum seq) ; last reflexivity.
     destruct (table_seq_sum seq') ; [simpl; f_equal; lia | reflexivity].
   Qed.
     
   
-  Definition test_1_inv l seq (_ : val) : iProp Σ :=
-    (∃ i, ⌜table_seq_sum seq = Some i⌝
+  Definition test_1_inv l (seq: list (val * val)) (_ : val) : iProp Σ :=
+    (∃ i, ⌜table_seq_sum (seq.*2) = Some i⌝
           ∗ l ↦ #i)%I.
 
   Lemma test_1_inner M l k x seq a:
     int_table M ->
     permitted M (seq ++ [(k,x)]) ->
-    {{test_1_inv l seq a}} (λ: "k" "x", #l <- !#l + "x") k x {{v, test_1_inv l (seq ++ [(k,x)]) v }}.
+    {{test_1_inv l seq a}} (λ: "k" "x" <>, #l <- !#l + "x") k x a {{v, test_1_inv l (seq ++ [(k,x)]) v }}.
   Proof.
-    intros HiTab HPer. pose proof (int_table_permitted _ _ HiTab HPer) as Hseq.
+    intros HiTab [M' HRem]. pose proof (table_inv_removal _ _ _ _ _ HiTab HRem) as Hseq.
     rewrite fmap_app in Hseq. apply Forall_app in Hseq. destruct Hseq as [_ Hx]. 
     setoid_rewrite Forall_singleton in Hx. destruct Hx as [j Hj]. simpl in Hj. rewrite Hj.
     iIntros "!# HInv". iDestruct "HInv" as (i) "[% ?]".
-    assert (Hi: table_seq_sum seq = Some i) ; first assumption.
-    do 2 wp_lam. wp_load. wp_op. wp_store. iExists (i + j)%Z. iSplit.
-    - by rewrite table_seq_sum_app Hi.
+    assert (Hi: table_seq_sum (seq.*2) = Some i) ; first assumption.
+    do 3 wp_lam. wp_load. wp_op. wp_store. iExists (i + j)%Z. iSplit.
+    - by rewrite fmap_app table_seq_sum_app Hi.
     - iFrame.
   Qed.
-    
-  
+
+   
   Lemma test_1_spec :
     WP test_1 {{v, ⌜v = #3⌝}}%I.
   Proof.
@@ -247,15 +273,141 @@ Section Tests.
     wp_lam. wp_apply (insert_spec (const []) 1 t #1 with "HTable").
     iIntros "HTable".
     wp_lam. wp_apply (insert_spec _ 2 t #2 with "HTable").
-    iIntros "Htable". wp_lam.
+    iIntros "HTable". iDestruct "HTable" as (D data) "HTable". wp_lam.
     wp_alloc a. wp_lam.
-    set (I := (fun ps (_:val) => ⌜Forall (fun '(_, x) => exists i, x = #i) ps⌝
-                             ∗ a ↦ #( foldr (fun p y => match p.1 with #(LitInt x) => x | _ => 0 end + y)%Z 0 ps))%I).
-    Check (fold_impl_spec nat_hashable (<[2:=#2]> (<[1:=#1]> (const []))) I (λ: "k" "x", #a <- !(#a) + "x") t #0).
-    
+    set (M:= (<[2:=#2]> (<[1:=#1]> (const [])))).
+    wp_apply (fold_impl_spec nat_hashable M D data (test_1_inv a) (LamV "k" (λ: "x" <>, #a <- ! #a + "x")) t #() with "[-]").
+    intros. apply (test_1_inner M).
+    unfold int_table ; eauto using table_inv_insert, table_inv_empty. assumption.
+    iFrame. iExists 0. eauto.
+    iIntros (v seq) "[% [HTable HInv]]".
+    iDestruct "HInv" as (n) "[% Hl]".
+    assert (HSum: table_seq_sum (seq.*2) = Some n) ; first assumption.
+    wp_seq. wp_load. iPureIntro. f_equal.
+    assert (Hperm: seq.*2 ≡ₚ elementsM nat_hashable M {[1; 2]}).
+    {
+      apply elementsM_complete_permutation ; last assumption.
+      intros k?. unfold M,  base.insert, insertM_nat, insertM.
+      do 2 (rewrite decide_False ; last set_solver). reflexivity.
+    }
+    rewrite ->Hperm in HSum. simpl in HSum. injection HSum as <-. reflexivity.
+  Qed.
 
-    assert (∀ (k x : val) (seq : list (val * val)) (a' : language.val heap_lang),
-               permitted nat_hashable (<[2:=#2]> (<[1:=#1]> (const []))) (seq ++ [(k, x)])
-               → hoare.ht ⊤ (I seq a') ((λ: "k" "x", #a <- ! #a + "x")%V k x)
-                          (λ v : language.val heap_lang, I (seq ++ [(k, x)]) v)).
-    { iIntros. iIntros "!#".
+
+  Definition test_2 (t : val) : expr :=
+    fold_impl (λ: <> "x" "a", "x" + "a")%V t #0.
+
+(*  Definition int_table_sum M (D : listset_nodup nat) :=
+    collection_fold (fun k x => foldr (fun v x => match v with #(LitInt y) => x + y | _ => 0 end) 0 (M k) + x)%Z 0 D.
+  
+  Lemma test_2_spec M D data t :
+    int_table M ->
+    {{{TableInState nat_hashable M D data t}}} test_2 t {{{RET #(int_table_sum M D) ; TableInState nat_hashable M D data t}}}.
+  Proof.
+  Admitted.*)
+  
+  Lemma test_2_spec M D data t :
+    int_table M ->
+    {{{TableInState nat_hashable M D data t}}}
+      test_2 t
+      {{{x, RET #x ; ⌜(table_seq_sum (elementsM nat_hashable M D)) = Some x⌝ ∗
+                     TableInState nat_hashable M D data t}}}.
+  Proof.
+    iIntros (HiTab Φ) "HTable HΦ".
+    iAssert (⌜is_domain nat_hashable D M⌝%I) as "%".
+    { by iDestruct "HTable" as "[_ [_ [_ [_ [? _]]]]]". }
+    wp_apply (fold_impl_spec nat_hashable M D data (fun seq v => ∃ x, ⌜table_seq_sum (seq.*2) = Some x⌝ ∗ ⌜v = #x⌝)%I with "[HTable]").
+    - intros k x seq a [? HRem].
+      iIntros "!# HInv".
+      iDestruct "HInv" as (x') "[% %]". iSimplifyEq.
+      pose proof (table_inv_removal _ _ _ _ _ HiTab HRem) as Hseq.
+      rewrite fmap_app in Hseq. apply Forall_app in Hseq. simpl in Hseq.
+      rewrite ->Forall_singleton in Hseq. destruct Hseq as [Hseq [xz ->]].
+      do 3 wp_lam. wp_op. iExists (xz + x')%Z. iSplit ; iPureIntro.
+      rewrite fmap_app table_seq_sum_app (_:table_seq_sum (seq.*2) = Some x') /=; last assumption.
+      f_equal. lia. reflexivity.
+    - eauto.
+    - iIntros (v seq) "[% [HTable HInv]]".
+      iDestruct "HInv" as (x) "[% %]". iSimplifyEq. iApply "HΦ".
+      iSplit. by rewrite -elementsM_complete_permutation.
+      iAssumption.
+  Qed.
+
+  
+  Definition test_3 : expr :=
+    let: "t" := create_impl #10 in
+    insert "t" #1 #1 ;;
+    insert "t" #2 #2 ;;
+    let: "a" := ref #0 in
+    (rec: "loop" "c" :=
+       match: "c" #() with
+         NONE     => !"a"
+       | SOME "p" => "a" <- !"a" + Snd (Fst "p") ;;
+                     "loop" (Snd "p")
+       end) (cascade_impl "t").
+
+  Lemma test_3_spec :
+    WP test_3 {{ v, ⌜v = #3⌝ }}%I.
+  Proof.
+    assert (H10: 10 > 0) ; first lia.
+    unfold test_3. rewrite (_:10%Z = 10%nat) ; last lia.
+    wp_bind (create_impl _). iApply wp_wand.
+    iApply (create_impl_spec nat_hashable _ H10).
+    iIntros (t) "HTable".
+    wp_lam. wp_apply (insert_spec (const []) 1 t #1 with "HTable").
+    iIntros "HTable".
+    wp_lam. wp_apply (insert_spec _ 2 t #2 with "HTable").
+    iIntros "HTable". iDestruct "HTable" as (D data) "HTable". wp_lam.
+    wp_alloc a. wp_lam.
+    set (M:= (<[2:=#2]> (<[1:=#1]> (const [])))).
+    iAssert (⌜is_domain _ D M⌝%I) as "%".
+    { by iDestruct "HTable" as "[_ [_ [_ [_ [% _]]]]]". }
+    wp_apply (cascade_impl_spec with "HTable").
+    iIntros (c) "[% HTable]". assert (Hcas: is_cascade nat_hashable c [] M data t) ; first assumption.
+    assert (Hloop: forall x seq,
+               table_seq_sum (seq.*2) = Some x ->
+               is_cascade nat_hashable c seq M data t ->
+               TableInState nat_hashable M D data t -∗ a ↦ #x -∗
+               WP (rec: "loop" "c" := match: "c" #() with
+                                        NONE => ! #a
+                                      | SOME "p" => #a <- ! #a + Snd (Fst "p") ;;
+                                                    "loop" (Snd "p")
+                                      end) c
+               {{ v, ⌜exists x seq, complete M seq /\ table_seq_sum (seq.*2) = Some x /\ v = #x⌝ }}).
+    { clear Hcas.
+      intros i seq Hi Hcas. clear H1.
+      iLöb as "IH" forall (c i seq Hi Hcas).
+      iIntros "HTable Ha".
+      wp_rec. wp_apply (is_cascade_spec with "HTable") ; first exact Hcas.
+      iIntros (? k x c') "[HTable [[% %]|[% [% %]]]]".
+      - simplify_eq. wp_match. wp_load. iPureIntro. exists i, seq. auto.
+      - simplify_eq. simpl.
+        assert (permitted M (seq ++ [(k, x)])) as [M' HRem] ; first assumption.
+        assert (HiTab:int_table M).
+        { unfold int_table, table_inv, M, base.insert, insertM_nat, insertM. intro k'.
+          case_decide ; last case_decide.
+          - rewrite decide_False. apply Forall_singleton. exists 2. reflexivity.
+            simplify_eq. discriminate.
+          - apply Forall_singleton. exists 1. reflexivity.
+          - by apply Forall_nil.
+        }
+        eapply table_inv_removal in HiTab ; last exact HRem.
+        rewrite fmap_app in HiTab. apply Forall_app in HiTab.
+        destruct HiTab as [_ Hx]. simpl in Hx. rewrite ->Forall_singleton in Hx.
+        destruct Hx as [j ->].
+        wp_match. wp_load. do 2 wp_proj. wp_op. wp_store. wp_proj.
+        iApply ("IH" $! _ (i + j)%Z (seq ++ [(k , #j)]) with "[] [] HTable Ha").
+        by rewrite fmap_app table_seq_sum_app Hi /=. done.
+    }
+    iApply (wp_wand with "[-]"). by iApply (Hloop 0 [] with "HTable [-]").
+    iIntros (v) "%".
+    assert (∃ (x : Z) (seq : list (val * val)), complete M seq ∧ table_seq_sum (seq.*2) = Some x ∧ v = #x) as [x [seq [Hcom [Hsum ->]]]] ; first assumption.
+    
+    assert (HPerm:seq.*2 ≡ₚ elementsM nat_hashable M {[1 ; 2]}).
+    { apply elementsM_complete_permutation ; last done.
+      intros k Hk. unfold M, base.insert, insertM_nat, insertM.
+      rewrite decide_False. rewrite decide_False. reflexivity.
+      all : set_solver.
+    }    
+    rewrite ->HPerm in Hsum. simpl in Hsum. injection Hsum as <-. done.
+  Qed.
