iterators/util.v
@@ -1,115 +1,136 @@
 From mathcomp Require Import ssreflect.
 From iris.prelude Require Import fin_collections listset_nodup.
 
-Definition collection_sum_with `{Elements A C} (f : A -> nat) : C -> nat :=
-      collection_fold (fun a n => n + f a) 0.
- 
- Instance collection_sum_with_proper `{FinCollection A C} (f : A -> nat) : Proper ((≡) ==> (=)) (collection_sum_with f : C -> nat).
- Proof.
-   unfold collection_sum_with.
-   apply (collection_fold_proper).
-   apply eq_equivalence.
-   solve_proper.
-   intros. lia.
- Qed.
- 
- Lemma collection_sum_with_empty `{FinCollection A C} f :
-   collection_sum_with f ∅ = 0.
- Proof.
-      unfold collection_sum_with, collection_fold. simpl.
-      rewrite elements_empty. done.
- Qed.
- 
- Lemma collection_sum_with_singleton_union `{FinCollection A C} x D f :
-   x ∉ D ->
-   collection_sum_with f ({[x]} ∪ D) = f x + collection_sum_with f D.
- Proof.
-   intro. 
-   unfold collection_sum_with, collection_fold. simpl.
-   rewrite (foldr_permutation (=) (λ (a : A) (n : nat), n + f a) 0 _ (elements ({[x]} ∪ D))(x :: elements D)) ; [|intros ; lia|].
-   simpl. lia.
-   by apply elements_union_singleton.  
- Qed.
- 
- Lemma collection_sum_with_subseteq_le `{FinCollection A C} `{forall x D, Decision (x ∈ D)} (D1 D2 : C) f :
-   D1 ⊆ D2 ->
-   collection_sum_with f D1 ≤ collection_sum_with f D2. 
- Proof.
-   apply (collection_ind
-            (fun D1 => forall D2,
-                 D1 ⊆ D2 ->
-                 collection_sum_with f D1 ≤ collection_sum_with f D2)). 
-   { intros ? ? Heq. apply forall_proper. intros.
-     rewrite subseteq_proper ; [|done..].
-     by rewrite (collection_sum_with_proper f _ _ Heq ).
-   }
-   - clear D1 D2.
-     intros D2 _. rewrite collection_sum_with_empty. lia.
-   - clear D1 D2.
-     intros x D1 Hx IH D2 Hsubset.
-     rewrite (union_difference {[x]} D2) ; [|set_solver].
-     rewrite collection_sum_with_singleton_union.
-     rewrite collection_sum_with_singleton_union.
-     assert (D1 ⊆ D2 ∖ {[x]}) as Hsubset'. set_solver.
-     specialize (IH (D2 ∖ {[x]}) Hsubset').
-     lia. set_solver. assumption.
- Qed.
- Lemma collection_sum_with_union `{FinCollection A C} `{forall x D, Decision (x ∈ D)} D1 D2 f :
-   collection_sum_with f (D1 ∪ D2) =
-   (collection_sum_with f D1 + collection_sum_with f D2) - collection_sum_with f (D1 ∩ D2).
- Proof.
-   apply (collection_ind (fun D => collection_sum_with f (D ∪ D2) =
-                                   (collection_sum_with f D + collection_sum_with f D2) - collection_sum_with f (D ∩ D2))).
-   {
-     intros X Y ?. rewrite union_proper ; [|done..].
-     rewrite intersection_proper ; [|done..].
-       by rewrite (collection_sum_with_proper _ X Y).
-   }
-   - rewrite intersection_empty_l union_empty_l collection_sum_with_empty .
-     lia.
-   - intros x D HnIn IH.
-     rewrite collection_sum_with_singleton_union ; [|assumption].
-     
-     destruct (decide (x ∈ D2)) as [HD2|HD2].
-     + rewrite {1}[{[x]} ∪ D]union_comm -union_assoc (subseteq_union_1 {[x]} D2).
-       rewrite intersection_union_r. rewrite (subseteq_intersection_1 {[x]} D2).
-       rewrite collection_sum_with_singleton_union.
-       rewrite IH. lia.
-       rewrite not_elem_of_intersection. by left.
-       apply elem_of_subseteq_singleton. assumption.
-       apply elem_of_subseteq_singleton. assumption.
-     + rewrite -union_assoc.
-       rewrite collection_sum_with_singleton_union.
-       rewrite intersection_union_r. rewrite (_:{[x]} ∩ D2 ≡ ∅).
-       rewrite union_empty_l. rewrite IH.
-       pose proof (collection_sum_with_subseteq_le (D ∩ D2) D f (intersection_subseteq_l _ _)).
-       lia. set_solver. set_solver.
- Qed.
- 
- Lemma collection_sum_with_domains `{FinCollection A C} D f g :
-   (forall x, x ∈ D -> f x = g x) ->
-   collection_sum_with f D = collection_sum_with g D.
- Proof.
-   apply (collection_ind (fun D => (forall x, x ∈ D -> f x = g x) ->
-                                   collection_sum_with f D = collection_sum_with g D)).
-   { intros ? ? Heq.
-     rewrite (collection_sum_with_proper f _ _ Heq).
-     rewrite (collection_sum_with_proper g _ _ Heq).
-     split. intros Hother Hdom. apply Hother. intro. rewrite elem_of_proper ;[|done..]. apply Hdom.
-     intros Hother Hdom. apply Hother. intro. rewrite elem_of_proper ;[|done..]. apply Hdom.
-   }
-   - intro. rewrite collection_sum_with_empty.
-     symmetry. apply collection_sum_with_empty.
-   - clear D. intros x D Hx IH Hdom. 
-     rewrite collection_sum_with_singleton_union ; [|assumption].
-     rewrite collection_sum_with_singleton_union ; [|assumption].
-     rewrite Hdom ; [|set_solver].
-     rewrite IH. done.
-     intros ? ?. apply Hdom. set_solver.
- Qed.        
+Lemma collection_fold_union_singleton `{FinCollection A C} {B} f (b : B) (x : A) (X : C)
+      `{!Equivalence R} `{!Proper ((=) ==> R ==> R) f} :
+  (∀ a1 a2 b, R (f a1 (f a2 b)) (f a2 (f a1 b))) ->
+  x ∉ X ->
+  R (collection_fold f b ({[x]} ∪ X)) (f x (collection_fold f b X)).
+Proof.
+  assert (HProper: Proper (eq ==> R ==> R) f) ; first assumption.
+  intros Hf ?.
+  rewrite /collection_fold /=.
+  assert (Proper ((≡ₚ) ==> R) (foldr f b)).
+  { intro. apply foldr_permutation. typeclasses eauto. intro. by apply HProper. assumption. }
+  rewrite elements_union_singleton /=; last assumption. reflexivity.
+Qed.
 
- Instance listset_nodup_dec_elem_of `{EqDecision A} x (C : listset_nodup A) : Decision (x ∈ C) :=
-   elem_of_list_dec x (elements C).
+Lemma collection_fold_domains `{FinCollection A C} {B} (b : B) X f g `{!Equivalence R}
+      `{!Proper ((=) ==> R ==> R) f} `{!Proper ((=) ==> R ==> R) g}:
+  (∀ a1 a2 b, R (f a1 (f a2 b)) (f a2 (f a1 b))) ->
+  (∀ a1 a2 b, R (g a1 (g a2 b)) (g a2 (g a1 b))) ->
+  (forall a b1 b2, R b1 b2 -> a ∈ X -> R (f a b1) (g a b2)) ->
+  R (collection_fold f b X) (collection_fold g b X).
+Proof.
+  intros.
+  apply (collection_ind
+           (fun X => (forall a b1 b2, R b1 b2 -> a ∈ X -> R (f a b1) (g a b2)) ->
+                     R (collection_fold f b X) (collection_fold g b X))) ; last assumption.
+  {
+    intros ?? Heq. rewrite (collection_fold_proper _ _ _ _ _ _ Heq).
+    rewrite (collection_fold_proper _ _ _ _ _ _ Heq).
+      split ; intros Hyp ? ; apply Hyp ; intros ???? ; [rewrite Heq |rewrite -Heq] ; eauto.
+      all : assumption.
+  }
+  - intros. by rewrite /collection_fold /= elements_empty. 
+  - intros ??? IH Hfg.
+    rewrite collection_fold_union_singleton ; [|assumption..].
+    rewrite collection_fold_union_singleton ; [|assumption..].
+    apply Hfg. apply IH. intros. apply Hfg. assumption. all: set_solver.
+Qed.
+
+Definition collection_sum_with `{Elements A C} (f : A -> nat) : C -> nat :=
+  collection_fold (fun a n => n + f a) 0.
+
+Instance collection_sum_with_proper `{FinCollection A C} (f : A -> nat) : Proper ((≡) ==> (=)) (collection_sum_with f : C -> nat).
+Proof.
+  unfold collection_sum_with.
+  apply (collection_fold_proper).
+  apply eq_equivalence.
+  solve_proper.
+  intros. lia.
+ Qed.
+
+Lemma collection_sum_with_empty `{FinCollection A C} f :
+  collection_sum_with f ∅ = 0.
+Proof.
+  unfold collection_sum_with, collection_fold. simpl.
+  rewrite elements_empty. done.
+Qed.
+ 
+Lemma collection_sum_with_singleton_union `{FinCollection A C} x D f :
+  x ∉ D ->
+  collection_sum_with f ({[x]} ∪ D) = f x + collection_sum_with f D.
+Proof.
+  rewrite /collection_sum_with plus_comm.
+  apply (collection_fold_union_singleton (fun a n => n + f a)) ; [typeclasses eauto..|intros;lia].
+Qed.
+
+Lemma collection_sum_with_subseteq_le `{FinCollection A C} `{forall x D, Decision (x ∈ D)} (D1 D2 : C) f :
+  D1 ⊆ D2 ->
+  collection_sum_with f D1 ≤ collection_sum_with f D2. 
+Proof.
+  apply (collection_ind
+           (fun D1 => forall D2,
+                D1 ⊆ D2 ->
+                collection_sum_with f D1 ≤ collection_sum_with f D2)). 
+  { intros ? ? Heq. apply forall_proper. intros.
+    rewrite subseteq_proper ; [|done..].
+      by rewrite (collection_sum_with_proper f _ _ Heq ).
+  }
+  - clear D1 D2.
+    intros D2 _. rewrite collection_sum_with_empty. lia.
+  - clear D1 D2.
+    intros x D1 Hx IH D2 Hsubset.
+    rewrite (union_difference {[x]} D2) ; [|set_solver].
+    rewrite collection_sum_with_singleton_union.
+    rewrite collection_sum_with_singleton_union.
+    assert (D1 ⊆ D2 ∖ {[x]}) as Hsubset'. set_solver.
+    specialize (IH (D2 ∖ {[x]}) Hsubset').
+    lia. set_solver. assumption.
+Qed.
+Lemma collection_sum_with_union `{FinCollection A C} `{forall x D, Decision (x ∈ D)} D1 D2 f :
+  collection_sum_with f (D1 ∪ D2) =
+  (collection_sum_with f D1 + collection_sum_with f D2) - collection_sum_with f (D1 ∩ D2).
+Proof.
+  apply (collection_ind (fun D => collection_sum_with f (D ∪ D2) =
+                                  (collection_sum_with f D + collection_sum_with f D2) - collection_sum_with f (D ∩ D2))).
+  {
+    intros X Y ?. rewrite union_proper ; [|done..].
+    rewrite intersection_proper ; [|done..].
+      by rewrite (collection_sum_with_proper _ X Y).
+  }
+  - rewrite intersection_empty_l union_empty_l collection_sum_with_empty .
+    lia.
+  - intros x D HnIn IH.
+    rewrite collection_sum_with_singleton_union ; [|assumption].
+    
+    destruct (decide (x ∈ D2)) as [HD2|HD2].
+    + rewrite {1}[{[x]} ∪ D]union_comm -union_assoc (subseteq_union_1 {[x]} D2).
+      rewrite intersection_union_r. rewrite (subseteq_intersection_1 {[x]} D2).
+      rewrite collection_sum_with_singleton_union.
+      rewrite IH. lia.
+      rewrite not_elem_of_intersection. by left.
+      apply elem_of_subseteq_singleton. assumption.
+      apply elem_of_subseteq_singleton. assumption.
+    + rewrite -union_assoc.
+      rewrite collection_sum_with_singleton_union.
+      rewrite intersection_union_r. rewrite (_:{[x]} ∩ D2 ≡ ∅).
+      rewrite union_empty_l. rewrite IH.
+      pose proof (collection_sum_with_subseteq_le (D ∩ D2) D f (intersection_subseteq_l _ _)).
+      lia. set_solver. set_solver.
+Qed.
+
+Lemma collection_sum_with_domains `{FinCollection A C} D f g :
+  (forall x, x ∈ D -> f x = g x) ->
+  collection_sum_with f D = collection_sum_with g D.
+Proof.
+  intro. unfold collection_sum_with.
+  apply collection_fold_domains ; [typeclasses eauto..| | |] ; [(intros ; lia)..|auto].
+Qed.   
+
+Instance listset_nodup_dec_elem_of `{EqDecision A} x (C : listset_nodup A) : Decision (x ∈ C) :=
+  elem_of_list_dec x (elements C).
  
 
     
